NewList -> List + Import `newlib` modifications on NewList.ec
Sign-Off: François Dupressoir

theories/List.ec
@@ -5,664 +5,1636 @@
  * Distributed under the terms of the CeCILL-B-V1 license
  * -------------------------------------------------------------------- *)
 
-require import Int.
-require import Pred.
+(* This API has been mostly inspired from the [seq] library of the
+ * ssreflect Coq extension. *)
 
+(* -------------------------------------------------------------------- *)
+require import Fun Pred Option Pair Int.
+
+(* -------------------------------------------------------------------- *)
 type 'a list = [
   | "[]"
-  | (::) of 'a & 'a list ].
+  | (::) of  'a & 'a list
+].
 
-(*** Recursor and Derived Induction Principles *)
-(** Recursor *)
-op list_rect (v:'b) (f:'a -> 'a list -> 'b -> 'b) (xs:'a list) =
-  with xs = "[]"      => v
-  with xs = (::) x xs => f x xs (list_rect v f xs).
+op size (xs : 'a list) =
+  with xs = []      => 0
+  with xs = y :: ys => 1 + (size ys).
 
-(** Induction principles. *)
-lemma list_case_eq (P:'a list -> bool) (xs:'a list):
-  (xs = [] => P xs) => 
-  ((exists x' xs', xs = x'::xs') => P xs) =>
-  P xs.
-proof strict.
-elim/list_case xs=> //= x xs -> //.
-by exists x; exists xs.
-qed.
+lemma size_ge0 (s : 'a list): 0 <= size s.
+proof. by elim s => //= x s; smt. qed.
 
-lemma list_ind_eq (P:'a list -> bool):
-  (forall xs, xs = [] => P xs) =>
-  (forall xs x' xs', xs = x'::xs' => P xs' => P xs) =>
-  (forall xs, P xs).
-proof strict.
-intros=> P_nil P_cons; elim.
-  by apply P_nil.
-  by intros=> x' xs' P_xs'; apply (P_cons (x'::xs') x' xs').
-qed.
+lemma size_eq0 (s : 'a list): (size s = 0) <=> (s = []).
+proof. by case s => //=; smt. qed.
 
-(*** Destructors (partially specified) *)
-(** Head *)
-op hd: 'a list -> 'a.
-axiom hd_cons (x:'a) xs: hd (x::xs) = x.
+(* -------------------------------------------------------------------- *)
+op head (z0 : 'a) (s : 'a list) =
+  with s = []     => z0
+  with s = x :: s => x.
 
-(** Tail *)
-op tl: 'a list -> 'a list.
-axiom tl_cons (x:'a) xs: tl (x::xs) = xs.
+lemma head_nil (z0 : 'a): head z0 [] = z0.
+proof. by []. qed.
 
-(** Lemma *)
-lemma cons_hd_tl (xs:'a list):
-  xs <> [] => xs = (hd xs)::(tl xs).
-proof strict.
-elim/list_case xs=> //= x xs.
-by rewrite hd_cons tl_cons.
-qed.
+lemma head_cons (z0 : 'a) x s: head z0 (x :: s) = x.
+proof. by []. qed.
 
-(*** Operators *)
-(** foldr *)
-op foldr (f:'a -> 'b -> 'b) (v:'b) (xs:'a list) =
-  with xs = "[]"      => v
-  with xs = (::) x xs => f x (foldr f v xs).
+(* -------------------------------------------------------------------- *)
+op ohead (s : 'a list) =
+  with s = []     => None
+  with s = x :: s => Some x.
 
-(** foldl *)
-op foldl (f:'a -> 'b -> 'b) (v:'b) (xs:'a list) =
-  with xs = "[]"      => v
-  with xs = (::) x xs => foldl f (f x v) xs.
+lemma ohead_nil: ohead [<:'a>] = None.
+proof. by []. qed.
 
-(** mem *)
-op mem (e:'a) (xs:'a list) =
-  with xs = "[]"      => false
-  with xs = (::) x xs => x = e \/ mem e xs.
+lemma ohead_cons (x : 'a) s: ohead (x :: s) = Some x.
+proof. by []. qed.
 
-(* alternate definitions: short-circuiting and foldr *)
-op memsc (e:'a) (xs:'a list) =
-  with xs = "[]"      => false
-  with xs = (::) x xs => x = e || memsc e xs.
+lemma head_ohead z0 (s : 'a list):
+  head z0 s = odflt z0 (ohead s).
+proof. by case: s. qed.
 
-lemma memsc_mem (e:'a) xs:
-  memsc e xs = mem e xs.
-proof strict.
-by elim xs=> //= x xs ->; rewrite ora_or.
-qed.
+lemma ohead_head z0 (s : 'a list): s <> [] =>
+  ohead s = Some (head z0 s).
+proof. by case: s. qed.
 
-lemma mem_foldr (e:'a) xs:
-  foldr (fun x b, x = e || b) false xs = mem e xs.
-proof strict.
-by elim xs=> //= x xs ->; rewrite ora_or.
-qed.
+(* -------------------------------------------------------------------- *)
+op behead (xs : 'a list) =
+  with xs = []      => []
+  with xs = y :: ys => ys.
 
-(* Lemmas *)
-lemma mem_cons_eq (x:'a) xs: mem x (x::xs) by [].
-lemma mem_cons_neq (x y:'a) xs: x <> y => mem y (x::xs) = mem y xs by [].
+lemma behead_nil: behead [<:'a>] = [].
+proof. by []. qed.
 
-lemma cons_mem (x y:'a) xs: mem y xs => mem y (x::xs) by [].
+lemma behead_cons (x : 'a) xs: behead (x :: xs) = xs.
+proof. by []. qed.
 
-lemma mem_hd (xs:'a list): mem (hd xs) xs <=> xs <> []
-by (split; smt).
+(* -------------------------------------------------------------------- *)
+lemma head_behead (xs : 'a list) z0:
+  xs <> [] =>
+  (head z0 xs) :: (behead xs) = xs.
+proof. by elim xs. qed.
 
-lemma nmem_nil (xs:'a list): (forall x, !mem x xs) <=> xs = [] by [].
+(* -------------------------------------------------------------------- *)
+(*                    Sequence catenation "cat"                         *)
+(* -------------------------------------------------------------------- *)
+op (++) (s1 s2 : 'a list) =
+  with s1 = []      => s2
+  with s1 = x :: s1 => x :: (s1 ++ s2).
 
-(** length *)
-op length (xs:'a list) =
-  with xs = "[]"      => 0
-  with xs = (::) x xs => 1 + length xs.
+op rcons (s : 'a list) (z : 'a) =
+  with s = []      => [z]
+  with s = x :: s' => x :: (rcons s' z).
 
-(* Notation *)
-op "`|_|":'a list -> int  = length.
+op last (x : 'a) s =
+  with s = []      => x
+  with s = y :: ys => last y ys.
 
-(* Lemmas *)
-lemma length_nneg (xs:'a list): 0 <= length xs
-by (elim xs=> //=; smt).
+lemma cat0s (s : 'a list): [] ++ s = s.
+proof. by []. qed.
 
-lemma length_cons_pos (x:'a) xs: 0 < length (x::xs)
-by (elim xs=> //=; smt).
+lemma cats0 (s : 'a list): s ++ [] = s.
+proof. by elim s=> //= x s ->. qed.
 
-lemma length0_nil (xs:'a list): length xs = 0 <=> xs = []
-by (elim xs=> //=; smt).
+lemma cat1s (x : 'a) (s : 'a list): [x] ++ s = x::s.
+proof. by []. qed.
 
-(** append *)
-op (++) (xs ys:'a list) =
-  with xs = "[]"      => ys
-  with xs = (::) x xs => x::(xs ++ ys).
+lemma cats1 (s : 'a list) (z : 'a): s ++ [z] = rcons s z.
+proof. by elim s => //= x s ->. qed.
 
-(* Lemmas *)
-lemma app_consC (x:'a) xs ys: (x::xs) ++ ys = x::(xs ++ ys)
-by elim xs.
+lemma cat_cons (x : 'a) s1 s2: (x :: s1) ++ s2 = x :: (s1 ++ s2).
+proof. by []. qed.
 
-lemma appl_nil (xs:'a list): xs ++ [] = xs
-by (elim xs=> //= x xs ->).
+lemma catA (s1 s2 s3 : 'a list): s1 ++ (s2 ++ s3) = (s1 ++ s2) ++ s3.
+proof. by elim s1=> //= x s1 ->. qed.
 
-lemma appA (xs ys zs:'a list):
-  xs ++ (ys ++ zs) = (xs ++ ys) ++ zs
-by (elim xs=> //= x xs->).
+lemma size_cat (s1 s2 : 'a list): size (s1 ++ s2) = size s1 + size s2.
+proof. by elim s1=> // x s1 /= ->; smt. qed.
 
-lemma length_app (xs ys:'a list):
-  length (xs ++ ys) = length xs + length ys
-by (elim xs=> //= xs ->; smt).
+lemma lastcons (x y : 'a) (s : 'a list): last x (y :: s) = last y s.
+proof. by []. qed.
 
-lemma mem_app (y:'a) xs ys:
-  mem y (xs ++ ys) = (mem y xs \/ mem y ys)
-by (elim xs=> //= x xs ->; rewrite -orbA).
+lemma lastcat (x : 'a) (s1 s2 : 'a list):
+  last x (s1 ++ s2) = last (last x s1) s2.
+proof. by elim s1 x=> //= x s1 ->. qed.
 
-(** rev *)
-op rev (xs:'a list) =
-  with xs = "[]"      => []
-  with xs = (::) x xs => rev xs ++ [x].
+lemma lastrcons (x y : 'a) (s : 'a list): last x (rcons s y) = y.
+proof. by elim s x=> //= x s ->. qed.
 
-op revacc (acc:'a list) (xs:'a list) =
-  with xs = "[]"      => acc
-  with xs = (::) x xs => revacc (x::acc) xs.
+lemma lastnonempty (x1 x2 : 'a) (s : 'a list):
+  s <> [] =>
+  last x1 s = last x2 s.
+proof. by case s. qed.
 
-lemma revacc_rev (xs:'a list):
-  revacc [] xs = rev xs.
-proof strict.
-rewrite -(appl_nil (rev xs)); generalize [].
-by elim xs=> //= x xs IH acc; rewrite IH -appA.
-qed.
+lemma size_rcons s (x : 'a):
+  size (rcons s x) = (size s) + 1.
+proof. by rewrite -cats1 size_cat /=. qed.
 
-(* Lemmas *)  
-lemma rev_app (xs ys:'a list):
-  rev (xs ++ ys) = (rev ys) ++ (rev xs).
-proof strict.
-elim xs=> //=.
-  by rewrite appl_nil.
-  by intros=> x xs ->; rewrite appA.
-qed.
+lemma cat_rcons (x : 'a) s1 s2 : rcons s1 x ++ s2 = s1 ++ x :: s2.
+proof. by rewrite -cats1 -catA. qed.
 
-lemma rev_rev (xs:'a list):
-  rev (rev xs) = xs.
-proof strict.
-by elim xs=> //= x xs; rewrite rev_app //= => ->.
-qed.
+lemma rcons_cat (x : 'a) s1 s2 : rcons (s1 ++ s2) x = s1 ++ rcons s2 x.
+proof. by rewrite -!cats1 catA. qed.
 
-lemma mem_rev (e:'a) xs:
-  mem e (rev xs) <=> mem e xs.
-proof strict.
-by elim xs=> //= x xs; rewrite mem_app -orbC=> ->.
-qed.
-
-lemma eq_rev (xs ys:'a list):
-  rev xs = rev ys <=> xs = ys
-by [].
-
-(** all *)
-pred all (p:'a -> bool) xs = forall x, mem x xs => p x.
-
-(* Direct inductive definition *)
-lemma all_nil (p:'a -> bool): all p [] by [].
-lemma all_cons (p:'a -> bool) x xs: all p (x::xs) = (p x /\ all p xs) by [].
-
-(* Lemmas *)
-lemma all_app (p:'a -> bool) xs ys: all p (xs ++ ys) = (all p xs /\ all p ys) by [].
-
-(** allb *)
-op allb (p:'a -> bool) (xs:'a list) =
-  with xs = "[]"      => true
-  with xs = (::) x xs => p x /\ allb p xs.
-
-op allbsc (p:'a -> bool) (xs:'a list) =
-  with xs = "[]"      => true
-  with xs = (::) x xs => p x && allbsc p xs.
-
-(* Lemmas *)
-lemma allbsc_allb (p:'a -> bool) (xs:'a list):
-  allbsc p xs <=> allb p xs
-by (elim xs=> //= x xs ->; rewrite anda_and).
-
-lemma allb_all (p:'a -> bool) xs:
-  allb p xs <=> all p xs
-by (elim xs=> //= x xs ->; rewrite all_cons).
-
-(** any *)
-pred any (p:'a -> bool) xs = exists x, mem x xs /\ p x.
-
-(* Direct inductive definition *)
-lemma any_nil (p:'a -> bool): !(any p []) by [].
-lemma any_cons (p:'a -> bool) x xs: any p (x::xs) = (p x \/ any p xs) by [].
-
-(* Lemmas *)
-lemma any_app (p:('a -> bool)) xs ys: any p (xs ++ ys) = (any p xs \/ any p ys) by [].
-
-(** anyb *)
-op anyb (p:'a -> bool) (xs:'a list) =
-  with xs = "[]"      => false
-  with xs = (::) x xs => p x \/ anyb p xs.
-
-op anybsc (p:'a -> bool) (xs:'a list) =
-  with xs = "[]"      => false
-  with xs = (::) x xs => p x || anybsc p xs.
-
-(* Lemmas *)
-lemma anybsc_anyb (p:'a -> bool) xs:
-  anybsc p xs <=> anyb p xs
-by (elim xs=> //= x xs ->; rewrite ora_or).
-
-lemma anyb_any (p:'a -> bool) xs: anyb p xs <=> any p xs
-by (elim xs=> //= x xs ->; rewrite any_cons).
-
-(** find *)
-require import Option.
-op find (p:'a -> bool) (xs:'a list) =
-  with xs = "[]"      => None
-  with xs = (::) x xs => if p x then Some x else find p xs.
-
-lemma find_in (p:'a -> bool) (xs:'a list):
-  any p xs <=> find p xs <> None.
+(* -------------------------------------------------------------------- *)
+(*                   rcons / induction principle                        *)
+(* -------------------------------------------------------------------- *)
+lemma nosmt last_ind (p : 'a list -> bool):
+  p [] => (forall s x, p s => p (rcons s x)) => forall s, p s.
 proof.
-  rewrite -anyb_any; elim xs=> //= x xs IH.
-  by case (p x).
+  move=> Hnil Hlast s; rewrite -(cat0s s).
+  elim s [] Hnil => [|x s2 IHs] s1 Hs1; first by rewrite cats0.
+  by rewrite -cat_rcons (IHs (rcons s1 x)) // Hlast.
 qed.
 
-lemma find_nin (p:'a -> bool) (xs:'a list):
-  all (predC p) xs <=> find p xs = None.
+(* -------------------------------------------------------------------- *)
+(*                        Sequence indexing                             *)
+(* -------------------------------------------------------------------- *)
+op nth x (xs : 'a list) n : 'a =
+  with xs = []      => x
+  with xs = y :: ys => if n = 0 then y else (nth x ys (n-1)).
+
+op onth (xs : 'a list) n : 'a option =
+  with xs = []      => None
+  with xs = y :: ys =>  if n = 0 then Some y else (onth ys (n-1)).
+
+lemma nth_onth (z : 'a) xs n: nth z xs n = odflt z (onth xs n).
+proof. by elim xs n => //=; smt. qed.
+
+lemma onth_nth (z : 'a) xs n:
+  0 <= n < size xs => onth xs n = Some (nth z xs n).
+proof. by elim xs n => //=; smt. qed.
+
+lemma nth_default (z : 'a) s n: size s <= n => nth z s n = z.
 proof.
-  rewrite -allb_all /predC; elim xs=> //= x xs IH.
-  by case (p x).
+  elim s n => //= x s IHs n; case (n = 0).
+    by move=> ->; smt.
+    by move=> _ _; rewrite IHs; smt.
 qed.
 
-lemma find_cor (p:'a -> bool) (xs:'a list) (a:'a):
-  find p xs = Some a =>
-  mem a xs /\ p a.
+lemma nth_neg (x0 : 'a) s n: n < 0 => nth x0 s n = x0.
+proof. elim s n => //=; smt. qed.
+
+lemma nth_cat (x0 : 'a) s1 s2 n:
+  nth x0 (s1 ++ s2) n = if n < size s1 then nth x0 s1 n else nth x0 s2 (n - size s1).
 proof.
-  move: a; elim xs=> //= x xs IH a.
-  case (p x)=> //=.
-  by move=> _ /IH [] -> ->.
+  case (n < 0) => [n_lt0|n_ge0]; first by smt.
+  by elim s1 n n_ge0; smt.
 qed.
 
-(** filter *)
-op filter (p:'a -> bool) (xs:'a list) =
-  with xs = "[]"      => []
-  with xs = (::) x xs => let rest = filter p xs in
-                         if p x then x::rest else rest.
+lemma nth_rcons x0 (s : 'a list) x n:
+  nth x0 (rcons s x) n =
+    if n < size s then nth x0 s n else if n = size s then x else x0.
+proof. elim s n; smt. qed.
 
-op revfilter (acc:'a list) (p:'a -> bool) (xs:'a list) =
-  with xs = "[]"      => acc
-  with xs = (::) x xs => if p x then revfilter (x::acc) p xs
-                                else revfilter acc p xs.
-
-(* Lemmas *)
-lemma revfilter_filter (p:'a -> bool) xs:
-  rev (revfilter [] p xs) = filter p xs.
-proof strict.
-rewrite -(rev_rev (filter p xs)); congr.
-rewrite -(appl_nil (rev (filter p xs))); generalize [].
-by elim xs=> //= x xs IH acc; case (p x)=> _; rewrite IH - ?appA.
+lemma eq_from_nth x0 (s1 s2 : 'a list):
+     size s1 = size s2
+  => (forall i, 0 <= i < size s1 => nth x0 s1 i = nth x0 s2 i)
+  => s1 = s2.
+proof.                        (* BUG: CHECKING IS TOO LONG *)
+  elim s1 s2 => [|x1 s1 IHs1] [|x2 s2] //=; first 2 smt.
+  move=> eq_szS h; cut eq_sz: size s1 = size s2 by smt.
+  cut := h 0 => /= ->; first smt. rewrite (IHs1 s2) // => i le_i_s1.
+  cut := h (i+1); smt.
 qed.
 
-lemma filter_cons_in (p:'a -> bool) x xs:
-  p x => filter p (x::xs) = x::(filter p xs)
-by [].
+(* -------------------------------------------------------------------- *)
+(*                       Sequence membership                            *)
+(* -------------------------------------------------------------------- *)
+op mem (s : 'a list) (z : 'a) =
+  with s = []      => false
+  with s = x :: s' => (z = x) \/ mem s' z.
 
-lemma filter_cons_nin (p:'a -> bool) x xs:
-  !(p x) => filter p (x::xs) = filter p xs
-by [].
+lemma in_nil (x : 'a): mem [] x = false.
+proof. by []. qed.
 
-lemma mem_filter (p:'a -> bool) e xs:
-  mem e (filter p xs) <=> (mem e xs /\ p e)
-by (elim xs=> //=; smt).
+lemma mem_eq0 (s : 'a list):
+  (forall x, ! mem s x) => s = [].
+proof. by case: s => [|x s] // h; have := h x. qed.
 
-lemma filter_app (p:'a -> bool) xs ys:
-  filter p (xs ++ ys) = filter p xs ++ filter p ys
-by (elim xs=> //= x xs ->; case (p x)).
+lemma in_nilE: mem [<:'a>] = pred0.
+proof. by apply fun_ext. qed.
 
-lemma length_filter (p:'a -> bool) xs:
-  length (filter p xs) <= length xs
-by (elim xs=> //=; smt).
+lemma in_cons y s (x : 'a): mem (y :: s) x <=> (x = y) \/ (mem s x).
+proof. by []. qed.
 
-lemma all_filter (p:'a -> bool) xs:
-  all p (filter p xs)
-by [].
+lemma mem_head (x : 'a) s: mem (x :: s) x.
+proof. by []. qed.
 
-lemma filter_leq (p q:'a -> bool) xs:
-  p <= q =>
-  forall x, mem x (filter p xs) => mem x (filter q xs)
-by [].
+lemma mem_behead (s : 'a list):
+  forall x, mem (behead s) x => mem s x.
+proof. by move=> x; case: s => //= y s ->. qed.
 
-(** map *)
-op map (f:'a -> 'b) (xs:'a list) =
-  with xs = "[]"      => []
-  with xs = (::) x xs => (f x)::(map f xs).
-
-(* Lemmas *)
-lemma map_in: forall (f:'a -> 'b) x xs,
-  mem x xs => mem (f x) (map f xs).
-by intros=> f x xs; elim/list_ind xs; smt.
+lemma mem_head_behead z0 (s : 'a list):
+  s <> [] =>
+  forall x, (x = (head z0 s) \/ mem (behead s) x) <=> mem s x.
+proof.
+  move=> /head_behead h; rewrite -(h z0) head_cons behead_cons.
+  by move=> x; rewrite in_cons.
 qed.
 
-lemma mapO: forall (f:'a -> 'b) (g:'b -> 'c) (h:'a -> 'c) xs,
-  (forall x, g (f x) = h x) =>
-  map g (map f xs) = map h xs.
-proof strict.
-by intros=> f g h xs fOg; elim/list_ind xs; smt.
+lemma mem_seq1 (x y : 'a): mem [y] x <=> (x = y).
+proof. by []. qed.
+
+lemma mem_seq2 (x y1 y2 : 'a):
+  mem [y1; y2] x <=> (x = y1 \/ x = y2).
+proof. by []. qed.
+
+lemma mem_seq3 (x y1 y2 y3 : 'a):
+  mem [y1; y2; y3] x <=> (x = y1 \/ x = y2 \/ x = y3).
+proof. by []. qed.
+
+lemma mem_seq4 (x y1 y2 y3 y4 : 'a):
+  mem [y1; y2; y3; y4] x <=> (x = y1 \/ x = y2 \/ x = y3 \/ x = y4).
+proof. by []. qed.
+
+lemma mem_cat (x : 'a) s1 s2:
+  mem (s1 ++ s2) x <=> mem s1 x \/ mem s2 x.
+proof. by elim s1 => //=; smt. qed.
+
+lemma mem_rcons s (y : 'a):
+  forall x, mem (rcons s y) x = mem (y :: s) x.
+proof. by move=> x; rewrite -cats1 /= !mem_cat /= orbC. qed.
+
+lemma mem_nth (x0 : 'a) s n : 0 <= n < size s => mem s (nth x0 s n).
+proof. by elim: s n => [|x s ih] //= n; smt. qed.
+
+(* -------------------------------------------------------------------- *)
+(*                  find, filter, count, has, all                       *)
+(* -------------------------------------------------------------------- *)
+op find ['a] (p : 'a -> bool) s =
+  with s = []      => 0
+  with s = x :: s' => if p x then 0 else find p s' + 1.
+
+op count ['a] (p : 'a -> bool) xs =
+  with xs = []      => 0
+  with xs = y :: ys => (int_of_bool (p y)) + (count p ys).
+
+op filter (p : 'a -> bool) xs =
+  with xs = []      => []
+  with xs = y :: ys => if p y then y :: filter p ys else filter p ys.
+
+lemma count_ge0 (p : 'a -> bool) s: 0 <= count p s.
+proof. by elim s=> //= x s; smt. qed.
+
+lemma count_size p (s : 'a list): count p s <= size s.
+proof. by elim s => //= x s; smt. qed.
+
+op has (p : 'a -> bool) xs =
+  with xs = []      => false
+  with xs = y :: ys => (p y) \/ (has p ys).
+
+op all (p : 'a -> bool) xs =
+  with xs = []      => true
+  with xs = y :: ys => (p y) /\ (all p ys).
+
+lemma hasP p (s : 'a list): has p s <=> (exists x, mem s x /\ p x).
+proof.
+  elim s => //= y s IHs; case (p y) => py.
+    by rewrite orTb /=; exists y; smt.
+  by rewrite orFb IHs; split; elim=> x []; smt.
 qed.
 
-lemma map_app: forall (f:'a -> 'b) xs ys,
-  map f (xs ++ ys) = map f xs ++ map f ys.
-proof strict.
-by intros f xs ys; elim/list_ind xs; smt.
+lemma allP p (s : 'a list):
+  all p s <=> (forall x, mem s x => p x).
+proof.
+  elim s=> //= x s [IH1 IH2]; split.
+    by elim=> _ h y []; [move=> -> // | apply IH1].
+  move=> h; split; [by apply h | apply IH2].
+  by move=> y y_in_s; apply h; right.
 qed.
 
-lemma length_map: forall (f:'a -> 'b) xs,
-  length (map f xs) = length xs.
-proof strict.
-by intros f xs; elim/list_ind xs; smt.
+lemma filter_pred0 (s : 'a list): filter pred0 s = [].
+proof. by elim s. qed.
+
+lemma filter_predT (s : 'a list): filter predT s = s.
+proof. by elim s => //= x s ->. qed.
+
+lemma filter_predI (p1 p2 : 'a -> bool) (s : 'a list):
+  filter (predI p1 p2) s = filter p1 (filter p2 s).
+proof.
+  elim s => //= x s IHs; rewrite IHs /predI.
+  by case (p2 x) => //=; case (p1 x) => //=.
 qed.
 
-(** revmap *)
-op revmap (acc:'b list) (f:'a -> 'b) (xs:'a list) =
-  with xs = "[]"      => acc
-  with xs = (::) x xs => revmap ((f x)::acc) f xs.
+lemma count_filter p (s : 'a list): count p s = size (filter p s).
+proof. by elim s => //= x s ->; case (p x). qed.
 
-(* Lemmas *)
-lemma revmap_map (f:'a -> 'b) (xs:'a list):
-  rev (revmap [] f xs) = map f xs.
-proof strict.
-rewrite -(rev_rev (map f xs)); congr.
-rewrite -(appl_nil (rev (map f xs))); generalize [].
-by elim xs=> //= x xs IH acc; rewrite IH - ?appA.
+lemma count_pred0 (s : 'a list): count pred0 s = 0.
+proof. by rewrite count_filter filter_pred0. qed.
+
+lemma count_predT (s : 'a list): count predT s = size s.
+proof. by rewrite count_filter filter_predT. qed.
+
+lemma count_predC p (s : 'a list):
+  count p s + count (predC p) s = size s.
+proof. elim s; smt. qed.
+
+lemma has_nil p : has p [<:'a>] <=> false.
+proof. by []. qed.
+
+lemma size_filter p (s : 'a list): size (filter p s) = count p s.
+proof. by elim: s => //= x s; case: (p x) => _ ->. qed.
+
+lemma has_count p (s : 'a list): has p s <=> (0 < count p s).
+proof. by elim s => //= x s -> /=; case (p x); smt. qed.
+
+lemma has_pred0 (s : 'a list): has pred0 s <=> false.
+proof. by rewrite has_count count_pred0. qed.
+
+lemma has_predT (s : 'a list): has predT s <=> (0 < size s).
+proof. by rewrite has_count count_predT. qed.
+
+lemma all_count p (s : 'a list): all p s <=> (count p s = size s).
+proof. by elim s => //= x s; case (p x) => _ /=; smt. qed.
+
+lemma all_pred0 (s : 'a list): all pred0 s <=> (size s = 0).
+proof. by rewrite all_count count_pred0 eq_sym. qed.
+
+lemma all_predT (s : 'a list): all predT s.
+proof. by rewrite all_count count_predT. qed.
+
+lemma all_predC p (s : 'a list): all (predC p) s = ! has p s.
+proof. by elim s => //= x s ->; rewrite /predC; case (p x). qed.
+
+lemma eq_filter p1 p2 (s : 'a list):
+  (forall x, p1 x <=> p2 x) => filter p1 s = filter p2 s.
+proof. by move=> h; elim s=> //= x l; rewrite h => ->. qed.
+
+lemma eq_count p1 p2 (s : 'a list):
+  (forall x, p1 x <=> p2 x) => count p1 s = count p2 s.
+proof. by move=> h; rewrite !count_filter (eq_filter _ p2). qed.
+
+lemma eq_has p1 p2 (s : 'a list):
+  (forall x, p1 x <=> p2 x) => has p1 s <=> has p2 s.
+proof. by move=> h; rewrite !has_count (eq_count _ p2). qed.
+
+lemma eq_all p1 p2 (s : 'a list):
+  (forall x, p1 x <=> p2 x) => all p1 s <=> all p2 s.
+proof. by move=> h; rewrite !all_count (eq_count _ p2). qed.
+
+lemma has_sym (s1 s2 : 'a list): has (mem s1) s2 <=> has (mem s2) s1.
+proof. smt. qed.
+
+lemma has_pred1 (z : 'a) s: has (pred1 z) s <=> mem s z.
+proof. smt. qed.
+
+lemma filter_all p (s : 'a list): all p (filter p s).
+proof. by elim s => //= x s IHs; case (p x). qed.
+
+lemma all_filterP p (s : 'a list): all p s <=> filter p s = s.
+proof.
+  split; last by move=> <-; apply filter_all.
+  by elim s => //= x s IHs [-> Hs]; rewrite IHs.
 qed.
 
-(** nth *)
-require import Pair.
+lemma filter_id p (s : 'a list): filter p (filter p s) = filter p s.
+proof. by apply all_filterP; apply filter_all. qed.
 
-op nth (xs:'a list) n =
-  with xs = "[]" => None
-  with xs = (::) x xs => if n = 0
-                         then Some x
-                         else nth xs (n - 1).
+lemma filter_cat p (s1 s2 : 'a list): filter p (s1 ++ s2) = filter p s1 ++ filter p s2.
+proof. by elim s1 => //= x s1 ->; case (p x). qed.
 
-(* Lemmas *)
-lemma nth_cons0 (x:'a) xs:
-  nth (x::xs) 0 = Some x
-by done.
+lemma filter_cons p x (s : 'a list):
+  filter p (x :: s) = if p x then x :: filter p s else filter p s.
+proof. by case: (p x)=> ->. qed.
 
-lemma nth_consN (x:'a) xs n:
-  n <> 0 =>
-  nth (x::xs) n = nth xs (n - 1)
-by rewrite //= -neqF=> ->.
+lemma filter_rcons p x (s : 'a list):
+  filter p (rcons s x) = if p x then rcons (filter p s) x else filter p s.
+proof. by rewrite -!cats1 filter_cat; case: (p x)=> -> /=; rewrite ?cats0. qed.
 
-(* Lemmas *)
-lemma nth_neg (xs:'a list) n: n < 0 => nth xs n = None.
-proof strict.
-generalize n; elim xs=> //= x xs IH n n_neg.
-cut ->: (n = 0) = false by smt.
-by rewrite //= IH; smt.
+lemma count_cat p (s1 s2 : 'a list): count p (s1 ++ s2) = count p s1 + count p s2.
+proof. by rewrite !count_filter filter_cat size_cat. qed.
+
+lemma has_cat p (s1 s2 : 'a list): has p (s1 ++ s2) <=> has p s1 \/ has p s2.
+proof. by elim s1 => //= x s1 IHs; rewrite IHs; smt. qed.
+
+lemma all_cat p (s1 s2 : 'a list): all p (s1 ++ s2) <=> all p s1 /\ all p s2.
+proof. by elim s1 => //= x s1 IHs; rewrite IHs. qed.
+
+lemma mem_filter (p : 'a -> bool) x s:
+  mem (filter p s) x <=> p x /\ (mem s x).
+proof. by elim s => //= y s IHs; smt. qed.
+
+lemma find_ge0 p (s : 'a list): 0 <= find p s.
+proof. elim s; smt. qed.
+
+lemma has_find p (s : 'a list): has p s <=> (find p s < size s).
+proof. elim s; smt. qed.
+
+lemma find_size p (s : 'a list): find p s <= size s.
+proof. elim s; smt. qed.
+
+lemma find_cat p (s1 s2 : 'a list):
+  find p (s1 ++ s2) = if has p s1 then find p s1 else size s1 + find p s2.
+proof. elim s1; smt. qed.
+
+lemma nth_find z0 p (s : 'a list): has p s => p (nth z0 s (find p s)).
+proof. elim s; smt. qed.
+
+(* -------------------------------------------------------------------- *)
+(*                              Lookup                                  *)
+(* -------------------------------------------------------------------- *)
+op index (x : 'a) = find (pred1 x).
+
+lemma index_cons x y (s : 'a list):
+  index x (y :: s) = if x = y then 0 else index x s + 1.
+proof. by rewrite (eq_sym x y). qed.
+
+lemma index_ge0 x (s : 'a list): 0 <= index x s.
+proof. by rewrite /index find_ge0. qed.
+
+lemma index_size x (s : 'a list): index x s <= size s.
+proof. by rewrite /index find_size. qed.
+
+lemma index_mem x (s : 'a list): (index x s < size s) = (mem s x).
+proof. by rewrite -has_pred1 has_find. qed.
+
+lemma nth_index z0 x (s : 'a list): mem s x => nth z0 s (index x s) = x.
+proof.
+  rewrite -has_pred1 => h; apply (nth_find z0 (pred1 x)) in h.
+  by move: h; rewrite /pred1 => {2}<-.
 qed.
 
-lemma nth_geq_len (xs:'a list) n: length xs <= n => nth xs n = None.
-proof strict.
-generalize n; elim xs=> //= x xs IH n n_geq_len.
-cut ->: (n = 0) = false by smt.
-by rewrite //= IH; smt.
+lemma index_cat x (s1 s2 : 'a list):
+ index x (s1 ++ s2) = if mem s1 x then index x s1 else size s1 + index x s2.
+proof. by rewrite /index find_cat has_pred1. qed.
+
+lemma index_head x (s : 'a list): index x (x :: s) = 0.
+proof. by []. qed.
+
+(* -------------------------------------------------------------------- *)
+(*                            drop, take                                *)
+(* -------------------------------------------------------------------- *)
+op drop n (xs : 'a list) =
+  with xs = []      => []
+  with xs = y :: ys =>
+    if n <= 0 then xs else drop (n-1) ys.
+
+lemma drop0 (s : 'a list): drop 0 s = s.
+proof. by elim s. qed.
+
+lemma drop_neg n (s : 'a list): n < 0 => drop n s = s.
+proof. by elim s => //= x s IHs n_lt0; smt. qed.
+
+lemma drop_oversize n (s : 'a list):
+  size s <= n => drop n s = [].
+proof. by elim s n; smt. qed.
+
+lemma drop_size (s : 'a list): drop (size s) s = [].
+proof. by rewrite drop_oversize. qed.
+
+lemma drop_cons n x (s : 'a list):
+  drop n (x :: s) = if 0 < n then drop (n-1) s else x :: s.
+proof. by rewrite /= lezNgt; case (0 < n). qed.
+
+lemma size_drop n (s : 'a list):
+  0 <= n => size (drop n s) = max 0 (size s - n).
+proof. by elim s n => //=; smt. qed.
+
+lemma drop_cat n (s1 s2 : 'a list):
+    drop n (s1 ++ s2) =
+      if n < size s1 then drop n s1 ++ s2 else drop (n - size s1) s2.
+proof. by elim s1 n => //=; smt. qed.
+
+lemma drop_size_cat n (s1 s2 : 'a list):
+  size s1 = n => drop n (s1 ++ s2) = s2.
+proof. by move=> <-; rewrite drop_cat subzz ltzz drop0. qed.
+
+lemma drop_nth (z0 : 'a) n s: 0 <= n < size s =>
+  drop n s = nth z0 s n :: drop (n+1) s.
+proof.
+  elim: s n=> [|x s ih] n []; 1: by elim: n => [|n _] hn //=; 1: smt.
+  by elim: n => [|n ge0_n _] /=; rewrite ?drop0 //= smt.
 qed.
 
-lemma nth_range (xs:'a list) n:
-  0 <= n < length xs =>
-  nth xs n <> None.
-proof strict.
-move: n; elim xs=> //=; first smt.
-intros=> x xs IH n n_range; case (n = 0)=> // neq0_n.
-by rewrite IH; smt.
+op take n (xs : 'a list) =
+  with xs = []      => []
+  with xs = y :: ys =>
+    if n <= 0 then [] else y :: take (n-1) ys.
+
+lemma take0 (s : 'a list): take 0 s = [].
+proof. by elim s. qed.
+
+lemma take_neg n (s : 'a list): n < 0 => take n s = [].
+proof. by elim s; smt. qed.
+
+lemma take_oversize n (s : 'a list):
+  size s <= n => take n s = s.
+proof. by elim s n; smt. qed.
+
+lemma take_size (s : 'a list): take (size s) s = s.
+proof. by rewrite take_oversize. qed.
+
+lemma take_cons n x (s : 'a list):
+  take n (x :: s) = if 0 < n then x :: take (n-1) s else [].
+proof. by rewrite /= lezNgt; case (0 < n). qed.
+
+lemma size_take n (s : 'a list):
+  0 <= n => size (take n s) = if n < size s then n else size s.
+proof. by elim s n => //=; smt. qed.
+
+lemma take_cat n (s1 s2 : 'a list):
+   take n (s1 ++ s2) =
+     if n < size s1 then take n s1 else s1 ++ take (n - size s1) s2.
+proof. by elim s1 n => //=; smt. qed.
+
+lemma take_size_cat n (s1 s2 : 'a list):
+  size s1 = n => take n (s1 ++ s2) = s1.
+proof. by move=> <-; rewrite take_cat subzz ltzz take0 cats0. qed.
+
+lemma take_nth (z0 : 'a) n s: 0 <= n < size s =>
+  take (n+1) s = rcons (take n s) (nth z0 s n).
+proof.
+  elim: s n=> [|x s ih] n []; 1: by elim: n => [|n _] hn //=; 1: smt.
+  by elim: n => [|n ge0_n _] /=; rewrite ?take0 //= smt.
 qed.
 
-lemma mem_nth (xs:'a list) (n:int):
-  0 <= n < length xs =>
-  mem (oget (nth xs n)) xs.
-proof strict.
-generalize n; elim xs=> //=; first smt.
-intros=> x xs IH n n_range; case (n = 0).
-  by rewrite oget_some=> _; left.
-  by intros=> neq0_n; right; rewrite IH; first smt.
+lemma cat_take_drop n (s : 'a list): take n s ++ drop n s = s.
+proof. by elim s n; smt. qed.
+
+lemma nth_drop (x0 : 'a) n s i:
+  0 <= n => 0 <= i => nth x0 (drop n s) i = nth x0 s (n + i).
+proof.
+  move=> n_ge0 i_ge0; case (n < size s) => [lt_n_s|le_s_n]; last smt.
+  rewrite -{2}(cat_take_drop n s) nth_cat size_take //; smt.
 qed.
 
-lemma mem_ex_nth (e:'a) (xs:'a list):
-  mem e xs =>
-  exists (n:int), 0 <= n < length xs /\ nth xs n = Some e.
-proof strict.
-elim xs=> //= x xs IH [x_e | e_in_xs].
-  by exists 0; split=> //=; smt.
-  by apply IH in e_in_xs; elim e_in_xs=> n [n_bnd nth_e];
-     exists (n + 1); smt.
+lemma nth_take (x0 : 'a) n s i:
+  0 <= n => i < n => nth x0 (take n s) i = nth x0 s i.
+proof.
+  move=> n_ge0 i_ge0; case (n < size s) => [lt_n_s|le_s_n]; last smt.
+  by rewrite -{2}(cat_take_drop n s) nth_cat size_take //; smt.
 qed.
 
-lemma nth_append_left (ys xs:'a list) (n:int):
-  0 <= n < length xs =>
-  oget (nth (xs ++ ys) n) = oget (nth xs n).
-proof strict.
-generalize n; elim xs=> //=; first smt.
-intros=> x xs IH n n_bnd; case (n = 0)=> //=.
-by intros=> neq0_n; rewrite IH; first smt.
+lemma splitPr (xs : 'a list) (x : 'a): mem xs x =>
+  exists s1, exists s2, xs = s1 ++ x :: s2.
+proof.
+  move=> x_in_xs; pose i := index x xs.
+  have lt_ip: i < size xs by rewrite /i index_mem.
+  exists (take i xs); exists (drop (i+1) xs).
+  rewrite -{1}@(cat_take_drop i) -@(nth_index x x xs) //.
+  by rewrite -drop_nth // index_ge0 lt_ip.
 qed.
 
-lemma nth_append_right (xs ys:'a list) (n:int):
-  length xs <= n < length xs + length ys =>
-  oget (nth (xs ++ ys) n) = oget (nth ys (n - length xs)).
-proof strict.
-generalize n; elim xs=> //= x xs IH n n_bnd.
-cut ->: (n = 0) = false by smt.
-by rewrite //= IH; smt.
+(* -------------------------------------------------------------------- *)
+(*                          Sequence shift                              *)
+(* -------------------------------------------------------------------- *)
+op rot n (s : 'a list) = drop n s ++ take n s.
+
+lemma rot0 (s : 'a list): rot 0 s = s.
+proof. smt. qed.
+
+lemma rot_neg n (s : 'a list): n < 0 => rot n s = s.
+proof. by move=> lt0_n; rewrite /rot !(drop_neg, take_neg) // cats0. qed.
+
+lemma size_rot n (s : 'a list): size (rot n s) = size s.
+proof. smt. qed.
+
+lemma rot_oversize n (s : 'a list): size s <= n => rot n s = s.
+proof. smt. qed.
+
+lemma rot_size (s : 'a list): rot (size s) s = s.
+proof. by apply rot_oversize. qed.
+
+lemma has_rot n (s : 'a list) p: has p (rot n s) = has p s.
+proof. by rewrite /rot has_cat orbC -has_cat cat_take_drop. qed.
+
+lemma rot_size_cat (s1 s2 : 'a list): rot (size s1) (s1 ++ s2) = s2 ++ s1.
+proof. by rewrite /rot take_size_cat ?drop_size_cat. qed.
+
+lemma mem_rot n (s : 'a list): forall x, mem (rot n s) x <=> mem s x.
+proof.
+  by move=> x; rewrite -{2}(cat_take_drop n s) /rot !mem_cat orbC.
 qed.
 
-(** nth_default *)
-op nth_default (xs:'a list) (dv:'a) n =
-  let r = nth xs n in
-  if (r <> None) then oget r
-                 else dv.
+op rotr n (s : 'a list) = rot (size s - n) s.
 
-(** count *)
-op count (e:'a) (xs:'a list) =
-  with xs = "[]"      => 0
-  with xs = (::) x xs => count e xs + ((x = e)?1:0).
+lemma rotK n: cancel<:'a list, 'a list> (rot n) (rotr n).
+proof. smt. qed.
 
-op countacc (acc:int) (e:'a) (xs:'a list) =
-  with xs = "[]"      => acc
-  with xs = (::) x xs => countacc (acc + ((x = e)?1:0)) e xs.
+lemma rot_inj n (s1 s2 : 'a list): rot n s1 = rot n s2 => s1 = s2.
+proof. by apply (can_inj (rot n) (rotr n)); apply rotK. qed.
 
-(* Lemmas *)
-lemma countacc_count (e:'a) xs:
-  countacc 0 e xs = count e xs.
-proof strict.
-cut ->: count e xs = count e xs + 0 by smt.
-elim xs 0 => //= x xs IH n; case (x = e).
-  by rewrite IH; smt.
-  by rewrite /= IH.
+lemma rot1_cons x (s : 'a list): rot 1 (x :: s) = rcons s x.
+proof. by rewrite /rot /= take0 drop0 -cats1. qed.
+
+lemma rot_to (s : 'a list) x:
+  mem s x => exists i s', rot i s = x :: s'.
+proof.
+  move=> s_x; pose i := index x s.
+  exists i; exists (drop (i + 1) s ++ take i s).
+  rewrite -cat_cons /i /rot => {i}; congr=> //=.
+  elim s s_x => //= y s IHs; case (x = y); smt.
 qed.
 
-lemma nosmt count_cons_eq (x:'a) xs: count x (x::xs) = 1 + count x xs by [].
-lemma nosmt count_cons_neq (x y:'a) xs: x <> y => count y (x::xs) = count y xs by [].
+(* -------------------------------------------------------------------- *)
+(*                    Equality up to permutation                        *)
+(* -------------------------------------------------------------------- *)
+op perm_eq ['a] (s1 s2 : 'a list) =
+  all (fun x, count (pred1 x) s1 = count (pred1 x) s2) (s1 ++ s2).
 
-lemma leq0_count (e:'a) (xs:'a list):
-  0 <= count e xs.
-proof strict.
-by elim xs=> //= x xs IH; smt.
+lemma perm_eqP (s1 s2 : 'a list):
+  perm_eq s1 s2 <=> (forall p, count p s1 = count p s2).
+proof.
+  rewrite /perm_eq allP /=; split; last by move=> h x _; apply h.
+  move=> eq_cnt1 a; cut ltzSz: forall z, z < z + 1 by smt.
+  (* FIX: negative occurence selector *)
+  cut {ltzSz} := ltzSz (count a (s1 ++ s2)); move: {1 3 4}a.
+  pose x := _ + 1; cut : 0 <= x by smt. move: x => {a}.
+  elim/Int.Induction.induction; first by smt.
+  move=> i i_ge0 IHi a le_ai; case (count a (s1 ++ s2) = 0).
+    by rewrite count_cat; smt.
+  rewrite neq_ltz ltzNge count_ge0 /=; rewrite -has_count hasP.
+  case=> x [s12x a_x]; pose a' := predD1 a x.
+  cut cnt_a': forall s, count a s = count (pred1 x) s + count a' s.
+    move=> s; rewrite count_filter -(count_predC (pred1 x)).
+    rewrite  2!count_filter -!filter_predI -!count_filter.
+    by congr; apply eq_count => y; delta.
+  by rewrite !cnt_a' (eq_cnt1 x) // (IHi a') //; smt.
 qed.
 
-lemma count_mem (e:'a) (xs:'a list):
-  0 <> count e xs <=> mem e xs.
-proof strict.
-elim xs=> //= x xs IH; case (x = e)=> /=.
-  smt.
-  by rewrite IH.
+lemma perm_eq_refl (s : 'a list): perm_eq s s.
+proof. by apply perm_eqP. qed.
+
+lemma perm_eq_sym (s1 s2 : 'a list): perm_eq s1 s2 <=> perm_eq s2 s1.
+proof. by rewrite !perm_eqP; smt. qed.
+
+lemma perm_eq_trans (s2 s1 s3 : 'a list):
+  perm_eq s1 s2 => perm_eq s2 s3 => perm_eq s1 s3.
+proof. by rewrite !perm_eqP => h1 h2 p; rewrite h1 h2. qed.
+
+lemma perm_eqlP (s1 s2 : 'a list):
+  perm_eq s1 s2 <=> (forall s, perm_eq s1 s <=> perm_eq s2 s).
+proof.
+  split; last by move=> ->; rewrite perm_eq_refl.
+  move=> h s; split; last by apply perm_eq_trans.
+  by apply perm_eq_trans; apply perm_eq_sym.
 qed.
 
-(** DONE *)
-(** unique *)
-op unique:'a list -> bool.
-axiom unique_nil: unique<:'a> [].
-axiom unique_cons: forall (x:'a) xs, unique (x::xs) = (unique xs /\ !mem x xs).
+lemma perm_eqlE (s1 s2 : 'a list):
+  perm_eq s1 s2 => forall s, perm_eq s1 s <=> perm_eq s2 s.
+proof. by move=> h; apply perm_eqlP. qed.
 
-(* Lemmas *)
-lemma unique_count: forall (xs:'a list),
-  unique xs <=> (forall x, count x xs <= 1).
-proof strict.
-intros=> xs; split.
-  elim/list_ind xs.
-    by intros=> h x {h} //=; smt.
-    intros=> x xs IH; rewrite unique_cons -count_mem;
-    simplify; intros=> [u_xs x_nin_xs] x'; case (x = x')=> x_x'.
-      by subst x'; rewrite -x_nin_xs; smt.
-      by rewrite /= IH.
-  elim/list_ind xs.
-    by intros=> h {h}; apply unique_nil.
-    intros=> x xs IH count_xs; rewrite unique_cons; split.
-     apply IH => x'. 
-     by cut _ : count x' xs <= count x' (x :: xs); smt.
-     by cut _ : count x (x :: xs) <= 1; smt.
+lemma perm_catC (s1 s2 : 'a list): perm_eq (s1 ++ s2) (s2 ++ s1).
+proof. by rewrite !perm_eqP => p; rewrite !count_cat; smt. qed.
+
+lemma perm_catCl (s1 s2 : 'a list):
+  forall s, perm_eq (s1 ++ s2) s <=> perm_eq (s2 ++ s1) s.
+proof. by rewrite -perm_eqlP perm_catC. qed.
+
+lemma perm_cat2l (s1 s2 s3 : 'a list):
+  perm_eq (s1 ++ s2) (s1 ++ s3) <=> perm_eq s2 s3.
+proof.
+  by rewrite !perm_eqP; split=> h p; cut := h p; rewrite !count_cat; smt.
 qed.
 
-(** rm *)
-op rm:'a -> 'a list -> 'a list.
-axiom rm_nil: forall (x:'a), rm x [] = [].
-axiom rm_cons: forall (y x:'a) xs, rm y (x::xs) = ((x = y) ? xs : (x::rm y xs)).
+lemma perm_cat2r (s1 s2 s3 : 'a list):
+  perm_eq (s2 ++ s1) (s3 ++ s1) <=> perm_eq s2 s3.
+proof. by do 2! rewrite perm_eq_sym perm_catCl; apply perm_cat2l. qed.
 
-(* Lemmas *)
-lemma nosmt rm_consE: forall (x:'a) xs, rm x (x::xs) = xs by [].
-lemma nosmt rm_consNE: forall (x y:'a) xs, x <> y => rm y (x::xs) = x::(rm y xs) by [].
+lemma perm_catCAl (s1 s2 s3 : 'a list):
+  forall s, perm_eq (s1 ++ s2 ++ s3) s <=> perm_eq (s2 ++ s1 ++ s3) s.
+proof. by rewrite -!perm_eqlP perm_cat2r perm_catC. qed.
 
-lemma length_rm: forall (x:'a) xs,
-  mem x xs =>
-  length (rm x xs) = length xs - 1.
-proof strict.
-intros=> x xs; elim/list_ind xs.
-  by apply absurd=> h {h} //=.
-  intros=> x' xs IH x_in_xs //=; case (x' = x)=> x_x'.
-    by subst x'; rewrite rm_consE; smt.
-    generalize x_in_xs; rewrite // rm_consNE //= => x_in_xs; rewrite IH //; smt.
+lemma perm_catAC (s1 s2 s3 : 'a list):
+  forall s, perm_eq ((s1 ++ s2) ++ s3) s <=> perm_eq ((s1 ++ s3) ++ s2) s.
+proof. by rewrite -perm_eqlP -!catA perm_cat2l perm_catCl perm_eq_refl. qed.
+
+lemma perm_catCA (s1 s2 s3 : 'a list):
+  forall s, perm_eq (s1 ++ s2 ++ s3) s <=> perm_eq (s2 ++ s1 ++ s3) s.
+proof. by rewrite -perm_eqlP; rewrite perm_cat2r perm_catC. qed.
+
+lemma perm_consCA (x y : 'a) s:
+  forall s', perm_eq (x :: y :: s) s' <=> perm_eq (y :: x :: s) s'.
+proof. by move=> s'; cut := perm_catCA [x] [y] s s'. qed.
+
+lemma perm_cons (x : 'a) s1 s2:
+  perm_eq (x :: s1) (x :: s2) <=> perm_eq s1 s2.
+proof. by move: (perm_cat2l [x]) => /= h; apply h. qed.
+
+lemma perm_eq_mem (s1 s2 : 'a list):
+  perm_eq s1 s2 => forall x, mem s1 x <=> mem s2 x.
+proof. by rewrite perm_eqP => h x; rewrite -!has_pred1 !has_count h. qed.
+
+lemma perm_eq_size (s1 s2 : 'a list):
+  perm_eq s1 s2 => size s1 = size s2.
+proof. by rewrite perm_eqP=> h; rewrite -!count_predT h. qed.
+
+lemma perm_eq_small (s1 s2 : 'a list):
+  size s2 <= 1 => perm_eq s1 s2 => s1 = s2.
+proof.
+  move=> s2_le1 eqs12; move: s2_le1 (perm_eq_mem s1 s2 _) => //.
+  move: (perm_eq_size s1 s2 _) => // {eqs12}.
+  case s2 => [|x []] //=; first last; last 2 smt.
+  case s1 => [|y []] //=; last smt.
+  by move=> h; cut := h x => /= ->.
 qed.
 
-lemma count_rm_in: forall (x:'a) (xs:'a list),
-  mem x xs =>
-  count x (rm x xs) = count x xs - 1.
-proof strict.
-intros=> x xs; generalize x; elim/list_ind xs=> x.
-  apply absurd=> _ //=.
-  intros=> xs IH y x'; rewrite rm_cons (fun_if (count y)); smt.
+(* -------------------------------------------------------------------- *)
+(*                         Element removal                              *)
+(* -------------------------------------------------------------------- *)
+op rem (z : 'a) s =
+  with s = []      => []
+  with s = x :: s' => if x = z then s' else x :: (rem z s').
+
+lemma rem_id (z : 'a) s: ! mem s z => rem z s = s.
+proof.
+  elim s => //= y s IHs; rewrite -nor; elim.
+  move=> neq_yz s_notin_z; rewrite IHs // (eq_sym y).
+  by cut ->: (z = y) <=> false.
 qed.
 
-lemma count_rm_nin: forall (x:'a) (xs:'a list),
-  !mem x xs =>
-  count x (rm x xs) = count x xs.
-proof strict.
-intros=> x xs; generalize x; elim/list_ind xs=> x.
-  intros=> h {h}; rewrite rm_nil //.
-  intros=> xs IH x' //=; smt.
+lemma perm_to_rem (z : 'a) s : mem s z => perm_eq s (z :: rem z s).
+proof.
+  elim s => //= y s IHs; rewrite eq_sym perm_eq_sym.
+  rewrite -ora_or; elim; first by move=> -> /=; rewrite perm_eq_refl.
+  rewrite -neqF => -> /= z_in_s; rewrite -(cat1s z) -(cat1s y) catA.
+  by rewrite perm_catCAl /= perm_cons perm_eq_sym IHs.
 qed.
 
-lemma count_rm_neq: forall (x y:'a) (xs:'a list),
-  y <> x =>
-  count x (rm y xs) = count x xs.
-proof strict.
-intros=> x y xs; elim/list_ind xs.
-  rewrite rm_nil //.
-  intros=> x' xs IH x_y; smt.
+lemma size_rem (x : 'a) s: mem s x => size (rem x s) = (size s) - 1.
+proof.
+  move=> h; apply perm_to_rem in h; apply perm_eq_size in h.
+  by rewrite h; smt.
 qed.
 
-theory PermutationLists.
-  (** Equality up to permutation *)
-  pred (<->) (xs xs':'a list) =
-    forall (x:'a), count x xs = count x xs'.
+lemma mem_rem (x : 'a) (s : 'a list):
+  forall y, mem (rem x s) y => mem s y.
+proof.
+  move=> y; elim: s=> [|z s ih] //=; case: (z = x).
+    by move=> _ ->. by move=> _ [-> | /ih ->].
+qed.
 
-  lemma perm_refl: forall (xs:'a list), xs <-> xs by [].
-  lemma perm_symm: forall (xs ys:'a list), xs <-> ys => ys <-> xs by [].
-  lemma perm_trans: forall (ys xs zs:'a list), xs <-> ys => ys <-> zs => xs <-> zs by [].
+lemma all_rem p (x : 'a) (s : 'a list): all p s => all p (rem x s).
+proof. by move=> /allP h; apply/allP=> y /mem_rem /h. qed.
 
-  lemma perm_nil: forall (xs:'a list),
-    xs <-> [] =>
-    xs = [].
-  proof strict.
-  intros=> xs; delta (<->) beta=> xs_nil;
-  cut h: forall (x:'a), count x xs = 0.
-    by intros=> x; rewrite xs_nil.
-  by apply nmem_nil=> x; rewrite -count_mem eq_sym //= h.
+(* -------------------------------------------------------------------- *)
+(*                        Element insertion                             *)
+(* -------------------------------------------------------------------- *)
+op insert (x : 'a) (s : 'a list) (n : int) =
+  take n s ++ x :: drop n s.
+
+op trim (xs : 'a list) (n : int) =
+  take n xs ++ (drop (n+1) xs).
+
+(* -------------------------------------------------------------------- *)
+lemma trim_neg (xs : 'a list) (n : int): n < 0 => trim xs n = xs.
+proof. smt. qed.
+
+lemma size_trim (xs : 'a list) (n : int): 0 <= n < size xs =>
+  size (trim xs n) = size xs - 1.
+proof. smt. qed.
+
+lemma trim_head (x : 'a) (xs : 'a list):
+  trim (x :: xs) 0 = xs.
+proof. smt. qed.
+
+lemma trim_tail (x : 'a) (xs : 'a list) (n : int): 0 <= n =>
+  trim (x :: xs) (n+1) = x :: trim xs n.
+proof. smt. qed.
+
+lemma trim_cat (xs ys : 'a list) (n : int): n < size (xs ++ ys) =>
+  trim (xs ++ ys) n =
+    if   n < size xs
+    then (trim xs n) ++ ys
+    else xs ++ trim ys (n - size xs).
+proof. by rewrite size_cat smt. qed.
+
+(* -------------------------------------------------------------------- *)
+(*                        Sequence reversal                             *)
+(* -------------------------------------------------------------------- *)
+op catrev (s1 s2 : 'a list) =
+  with s1 = []      => s2
+  with s1 = x :: s1 => catrev s1 (x :: s2).
+
+op rev (s : 'a list) = catrev s [].
+
+lemma catrev_catl (s t u : 'a list):
+  catrev (s ++ t) u = catrev t (catrev s u).
+proof. by elim s u => //= x s h u; rewrite h. qed.
+
+lemma catrev_catr (s t u : 'a list):
+  catrev s (t ++ u) = catrev s t ++ u.
+proof. by elim s t => //= x s IHs t; rewrite -IHs. qed.
+
+lemma catrevE (s t : 'a list): catrev s t = rev s ++ t.
+proof. by rewrite /rev -catrev_catr. qed.
+
+lemma rev_nil: rev [<:'a>] = [].
+proof. by rewrite /rev. qed.
+
+lemma rev_cons (x : 'a) s: rev (x :: s) = rcons (rev s) x.
+proof. by rewrite -cats1 -catrevE. qed.
+
+lemma rev1 (x : 'a): rev [x] = [x].
+proof. by []. qed.
+
+lemma size_rev (s : 'a list): size (rev s) = size s.
+proof.
+  elim s; first by rewrite /rev.
+  by move=> x s IHs; rewrite rev_cons size_rcons IHs /=; smt.
+qed.
+
+lemma rev_cat (s t : 'a list): rev (s ++ t) = rev t ++ rev s.
+proof. by rewrite /rev -catrev_catr /= -catrev_catl. qed.
+
+lemma rev_rcons s (x : 'a): rev (rcons s x) = x :: rev s.
+proof. by rewrite -cats1 rev_cat /rev /=. qed.
+
+lemma revK (s : 'a list): rev (rev s) = s.
+proof. by elim s; smt. qed.
+
+lemma mem_rev (s : 'a list):
+  forall x, mem (rev s) x = mem s x.
+proof.
+  move=> x; elim s; first by rewrite rev_nil.
+  by move=> y s IHs; rewrite rev_cons mem_rcons /= IHs.
+qed.
+
+lemma filter_rev p (s : 'a list): filter p (rev s) = rev (filter p s).
+proof.
+  elim: s => /= [|x s ih]; rewrite ?rev_nil // fun_if.
+  by rewrite !rev_cons filter_rcons ih.
+qed.
+
+lemma count_rev p (s : 'a list): count p (rev s) = count p s.
+proof. by rewrite -!size_filter filter_rev size_rev. qed.
+
+lemma has_rev p (s : 'a list): has p (rev s) = has p s.
+proof. by rewrite !has_count count_rev. qed.
+
+lemma all_rev p (s : 'a list): all p (rev s) = all p s.
+proof. by rewrite !all_count count_rev size_rev. qed.
+
+(* -------------------------------------------------------------------- *)
+(*                        Duplicate-freenes                             *)
+(* -------------------------------------------------------------------- *)
+op uniq (s : 'a list) =
+  with s = []      => true
+  with s = x :: s' => !(mem s' x) /\ uniq s'.
+
+lemma cons_uniq (x : 'a) s:
+  uniq (x :: s) <=> (!mem s x) /\ uniq s.
+proof. by []. qed.
+
+lemma cat_uniq (s1 s2 : 'a list):
+  uniq (s1 ++ s2) <=> uniq s1 /\ ! has (mem s1) s2 /\ uniq s2.
+proof.
+  elim s1 => [|x s1 IHs]; first by rewrite /= in_nilE has_pred0.
+  by rewrite has_sym /= IHs has_sym mem_cat => {IHs}; smt.
+qed.
+
+lemma uniq_catC (s1 s2 : 'a list): uniq (s1 ++ s2) = uniq (s2 ++ s1).
+proof. by rewrite !cat_uniq has_sym; smt. qed.
+
+lemma uniq_catCA (s1 s2 s3 : 'a list):
+  uniq (s1 ++ s2 ++ s3) <=> uniq (s2 ++ s1 ++ s3).
+proof.
+  by rewrite -!(uniq_catC s3) !(cat_uniq s3) uniq_catC !has_cat orbC.
+qed.
+
+lemma rcons_uniq s (x : 'a): uniq (rcons s x) <=> (!mem s x) /\ uniq s.
+proof. by rewrite -cats1 uniq_catC /=. qed.
+
+lemma filter_uniq (s : 'a list) p: uniq s => uniq (filter p s).
+proof. by elim s => //=; smt. qed.
+
+lemma rot_uniq n (s : 'a list): uniq (rot n s) = uniq s.
+proof. by rewrite /rot uniq_catC cat_take_drop. qed.
+
+lemma rev_uniq (s : 'a list): uniq (rev s) <=> uniq s.
+proof.
+  elim s => /=; [by rewrite rev_nil | move=> x s IHs].
+  by rewrite rev_cons -cats1 cat_uniq IHs /= mem_rev.
+qed.
+
+lemma rem_filter x (s : 'a list): uniq s =>
+  rem x s = filter (predC1 x) s.
+proof.
+  elim s => //= y s ih [y_notin_s /ih->]; rewrite /predC1.
+  case (y = x)=> //= <-; apply/eq_sym/all_filterP.
+  (* FIXME: non genuine unification failure *)
+     cut := all_predC (fun z => z = y) s => ->.
+  by cut := has_pred1 y => ->.
+qed.
+
+lemma index_uniq z0 i (s : 'a list):
+  0 <= i < size s => uniq s => index (nth z0 s i) s = i.
+proof. by elim: s i; smt. qed.
+
+lemma rem_uniq x s: uniq<:'a> s => uniq (rem x s).
+proof.                          (* FIXME: subseq *)
+  elim: s=> [|y s ih] //= [y_notin_s uq_s].
+  case: (y = x)=> // ne_xy; rewrite ih //=.
+  by move: y_notin_s; apply/contra => /mem_rem.
+qed.
+
+(* -------------------------------------------------------------------- *)
+(*                       Removing duplicates                            *)
+(* -------------------------------------------------------------------- *)
+op undup (s : 'a list) =
+  with s = []      => []
+  with s = x :: s' => if mem s' x then undup s' else x :: undup s'.
+
+lemma size_undup (s : 'a list): size (undup s) <= size s.
+proof. by elim s => //= x s IHs; smt. qed.
+
+lemma mem_undup (s : 'a list): forall x, mem (undup s) x = mem s x.
+proof. move=> x; elim s => //= y s IHs; smt. qed.
+
+lemma undup_uniq (s : 'a list): uniq (undup s).
+proof. by elim s => //= x s IHs; case (mem s x); smt. qed.
+
+lemma undup_id (s : 'a list): uniq s => undup s = s.
+proof. by elim s => //= x s IHs; smt. qed.
+
+lemma count_uniq_mem s (x : 'a):
+  uniq s => count (pred1 x) s = int_of_bool (mem s x).
+proof. elim s; smt. qed.
+
+lemma uniq_leq_size (s1 s2 : 'a list):
+  uniq s1 => (mem s1 <= mem s2) => size s1 <= size s2.
+proof.                          (* FIXME: test case for views *)
+  rewrite /Pred.(<=); elim s1 s2 => //.
+    by move=> s2 /=; rewrite size_ge0.
+  move=> x s1 IHs s2 [not_s1x Us1]; rewrite -(allP (mem s2)) /=.
+  case=> s2x; rewrite allP => ss12; cut := rot_to s2 x _ => //.
+  case=> i s3 def_s2; rewrite -(size_rot i s2) def_s2 /= lez_addl.
+  apply IHs => // y s1y; cut := ss12 y _ => //.
+  by rewrite -(mem_rot i) def_s2; case.
+qed.
+
+lemma leq_size_uniq (s1 s2 : 'a list):
+  uniq s1 => (mem s1 <= mem s2) => size s2 <= size s1 => uniq s2.
+proof.
+  rewrite /Pred.(<=); elim s1 s2 => [[] | x s1 IHs s2] //; first smt.
+  move=> Us1x; cut [not_s1x Us1] := Us1x; rewrite -(allP (mem s2)).  
+  case=> s2x; rewrite allP => ss12 le_s21.
+  cut := rot_to s2 x _ => //; case=> {s2x} i s3 def_s2.
+  move: le_s21; rewrite -(rot_uniq i) -(size_rot i) def_s2 /= lez_addl => le_s31.
+  cut ss13: forall y, mem s1 y => mem s3 y.
+    move=> y s1y; cut := ss12 y _ => //.
+    by rewrite -(mem_rot i) def_s2 in_cons; case=> // eq_yx.
+  rewrite IHs //=; move: le_s31; apply contraL; rewrite -ltzNge => s3x.
+  rewrite -lez_add1r; cut := uniq_leq_size (x::s1) s3 _ => //= -> //.
+  by apply (allP (mem s3)); rewrite /= s3x /= allP.
+qed.
+
+lemma uniq_size_uniq (s1 s2 : 'a list):
+     uniq s1 => (forall x, mem s1 x <=> mem s2 x)
+  => uniq s2 <=> (size s2 = size s1).
+proof.
+  move=> Us1 eqs12; split=> [Us2 | eq_sz12].
+    by rewrite eqz_leq !uniq_leq_size // => y; rewrite eqs12.
+  apply (leq_size_uniq s1) => //; first by move=> x; rewrite eqs12.
+  by rewrite eq_sz12 lezz.
+qed.
+
+lemma leq_size_perm (s1 s2 : 'a list):
+    uniq s1 => (mem s1 <= mem s2) => size s2 <= size s1
+  => (forall x, mem s1 x <=> mem s2 x) /\ (size s1 = size s2).
+proof.
+  move=> Us1 ss12 le_s21; cut Us2 := leq_size_uniq s1 s2 _ _ _ => //.
+  rewrite -anda_and; split=> [|h]; last by rewrite eq_sym -uniq_size_uniq.
+  move=> x; split; [by apply ss12 | move=> s2x; move: le_s21].
+  apply absurd => not_s1x; rewrite -ltzNge -lez_add1r.
+  cut := uniq_leq_size (x :: s1) => /= -> //=.
+  by rewrite /Pred.(<=) -(allP (mem s2)) /= s2x /= allP.
+qed.
+
+lemma perm_uniq (s1 s2 : 'a list):
+     (forall x, mem s1 x <=> mem s2 x) => size s1 = size s2
+  => uniq s1 <=> uniq s2.
+proof.
+  move=> Es12 Hs12; split=> Us.
+  by rewrite (uniq_size_uniq s1) // eq_sym.
+  by rewrite (uniq_size_uniq s2) // => y; rewrite Es12.
+qed.
+
+lemma perm_eq_uniq (s1 s2 : 'a list):
+  perm_eq s1 s2 => uniq s1 <=> uniq s2.
+proof.
+  move=> eq_s12; apply perm_uniq;
+    [by apply perm_eq_mem | by apply perm_eq_size].
+qed.
+
+lemma uniq_perm_eq (s1 s2 : 'a list):
+  uniq s1 => uniq s2 => (forall x, mem s1 x <=> mem s2 x) => perm_eq s1 s2.
+proof.
+  move=> Us1 Us2 eq12; rewrite /perm_eq allP => x _ /=.
+  by rewrite !count_uniq_mem // eq12.
+qed.
+
+lemma count_mem_uniq (s : 'a list):
+  (forall x, count (pred1 x) s = int_of_bool (mem s x)) => uniq s.
+proof.
+  move=> count1_s; cut Uus := undup_uniq s.
+  apply (perm_eq_uniq (undup s)); last by apply undup_uniq.
+  rewrite /perm_eq allP => x _ /=; rewrite count1_s.
+  by rewrite (count_uniq_mem (undup s) x) ?undup_uniq // mem_undup.
+qed.
+
+(* -------------------------------------------------------------------- *)
+(*                             Mapping                                  *)
+(* -------------------------------------------------------------------- *)
+op map (f : 'a -> 'b) xs =
+  with xs = []      => []
+  with xs = y :: ys => (f y) :: (map f ys).
+
+lemma eq_in_map (f1 f2 : 'a -> 'b) (s : 'a list):
+  (forall x, mem s x => f1 x = f2 x) <=> map f1 s = map f2 s.
+proof. elim: s => //= x s <-; smt. qed.
+
+lemma eq_map (f1 f2 : 'a -> 'b):
+     (forall x, f1 x = f2 x)
+  => forall s, map f1 s = map f2 s.
+proof. by move=> Ef; elim=> //= x s ->; rewrite Ef. qed.
+
+lemma map_f (f : 'a -> 'b) s x: mem s x => mem (map f s) (f x).
+proof. by elim: s => [|y s ih] //=; case=> [| /ih] ->. qed.
+
+lemma mapP ['a 'b] (f : 'a -> 'b) s y:
+  mem (map f s) y <=> (exists x, mem s x /\ y = f x).
+proof.
+  elim: s => [|x s ih] //=; case: (y = f x)=> //=.
+    by move=> ->; exists x.
+  move=> ne_yfx; split; 1: move/ih.
+    by case=> x' [hx' ->]; exists x'; rewrite hx'.
+  case=> x' [h ->>]; case: h; 1: by move=> ->>; move: ne_yfx.
+  by move=> x'_in_s; apply/ih; exists x'.
+qed.
+
+lemma uniq_map (f : 'a -> 'b) (s : 'a list):
+  uniq (map f s) => uniq s.
+proof.
+  elim: s=> //= x s ih [x1_notin_fs /ih] -> /=.
+  by apply/not_def=> /(map_f f).
+qed.
+
+lemma map_cons (f : 'a -> 'b) x s: map f (x :: s) = f x :: map f s.
+proof. by []. qed.
+
+lemma map_cat (f : 'a -> 'b) s1 s2:
+  map f (s1 ++ s2) = map f s1 ++ map f s2.
+proof. by elim s1 => [|x s1 IHs] //=; rewrite IHs. qed.
+
+lemma size_map (f : 'a -> 'b) s: size (map f s) = size s.
+proof. by elim s => [// | x s /= ->]. qed.
+
+lemma map_comp (f1 : 'b -> 'c) (f2 : 'a -> 'b) s:
+  map (f1 \o f2) s = map f1 (map f2 s).
+proof. by elim: s => //= x s ->. qed.
+
+lemma map_id (s : 'a list): map idfun s = s.
+proof. by elim: s => //= x s ->. qed.
+
+lemma id_map f (s : 'a list): (forall x, f x = x) => map f s = s.
+proof. by move=> h; rewrite -{2}@(map_id s); apply/eq_map. qed.
+
+lemma nth_map x1 x2 (f : 'a -> 'b) n s:
+  0 <= n < size s => nth x2 (map f s) n = f (nth x1 s n).
+proof. by elim s n; smt. qed.
+
+lemma onth_nth_map (s : 'a list) n: onth s n = nth None (map Some s) n.
+proof. by elim s n; smt. qed.
+
+lemma map_rcons (f : 'a -> 'b) s x:
+  map f (rcons s x) = rcons (map f s) (f x).
+proof. by rewrite -!cats1 map_cat. qed.
+
+lemma last_map (f : 'a -> 'b) s x:
+  last (f x) (map f s) = f (last x s).
+proof. by elim s x => //= x s ->. qed.
+
+lemma filter_map (f : 'a -> 'b) p s:
+  filter p (map f s) = map f (filter (preim f p) s).
+proof.
+  by elim s => //= x s IHs; rewrite (fun_if (map f)) /= IHs.
+qed.
+
+lemma has_map (f : 'a -> 'b) p s:
+  has p (map f s) = has (preim f p) s.
+proof. by elim s => //= x s ->. qed.
+
+lemma all_map (f :  'a -> 'b) p s:
+  all p (map f s) = all (preim f p) s.
+proof. by elim s => //= x s ->. qed.
+
+lemma count_map (f : 'a -> 'b) p s:
+  count p (map f s) = count (preim f p) s.
+proof. by elim s => //= x s ->. qed.
+
+lemma map_take (f : 'a -> 'b) n s:
+  map f (take n s) = take n (map f s).
+proof.
+  elim s n => //= x s IHs n.
+  by case (n <= 0) => // _; rewrite IHs.
+qed.
+
+lemma map_drop (f : 'a -> 'b) n s:
+  map f (drop n s) = drop n (map f s).
+proof.
+  elim s n => //= x s IHs n.
+  by case (n <= 0) => // _; rewrite IHs.
+qed.
+
+lemma map_rev (f : 'a -> 'b) s:
+  map f (rev s) = rev (map f s).
+proof. elim s; first by rewrite rev_nil. smt. qed.
+
+lemma perm_eq_map (f : 'a -> 'b) (s1 s2 : 'a list):
+  perm_eq s1 s2 => perm_eq (map f s1) (map f s2).
+proof.
+  move=> h; apply/perm_eqP=> p; rewrite !count_map.
+  by apply/perm_eqP.
+qed.
+
+lemma map_inj_in_uniq (f : 'a -> 'b) s:
+     (forall x y, mem s x => mem s y => f x = f y => x = y)
+  => uniq (map f s) <=> uniq s.
+proof.
+  elim: s => // x s ih injf /=; rewrite ih /=.
+    by move=> x' y' sx' sy'; apply/injf=> /=; rewrite ?(sx', sy').
+  case: (uniq s) => //= uniq_s; split=> h; 2: by apply/map_f.
+  move/mapP: h => [x'] [x'_in_s eq_fxx']; rewrite @(injf x x') //.
+  by rewrite mem_behead.
+qed.
+
+lemma mem_map_fst (xs : ('a * 'b) list) (x : 'a):
+  mem (map fst xs) x <=> (exists y, mem xs (x,y)).
+proof.
+  rewrite @(mapP fst); split; case=> [[x' y] [h ->]|y h].
+    by exists y. by exists (x, y).
+qed.
+
+lemma mem_map_snd (xs : ('a * 'b) list) (y : 'b):
+  mem (map snd xs) y <=> (exists x, mem xs (x,y)).
+proof.
+  rewrite @(mapP snd); split; case=> [[x y'] [h ->]|x h].
+    by exists x. by exists (x, y).
+qed.
+
+lemma nth_index_map (z0 : 'a) (f : 'a -> 'b) (s : 'a list) x:
+     (forall x y, mem s x => mem s y => f x = f y => x = y)
+  => mem s x => nth z0 s (index (f x) (map f s)) = x.
+proof.
+  elim: s => //= y s ih inj_f s_x; rewrite index_cons.
+  case: (f x = f y) => eqf /=; 1: by apply/eq_sym/inj_f.
+  move: s_x eqf; case: (x = y)=> //= ne_xy s_x _.
+  rewrite addz1_neq0 1:index_ge0 //= addAzN ih //.
+  by move=> x' y' s_x' s_y'; apply/inj_f; rewrite ?(s_x', s_y').
+qed.
+
+(* -------------------------------------------------------------------- *)
+(*                         Partial mapping                              *)
+(* -------------------------------------------------------------------- *)
+op pmap ['a 'b] (f : 'a -> 'b option) (s : 'a list) =
+  with s = []     => []
+  with s = x :: s =>
+    if f x = None then pmap f s else oget (f x) :: pmap f s.
+
+(* -------------------------------------------------------------------- *)
+(*                          Index sequence                              *)
+(* -------------------------------------------------------------------- *)
+theory Iota.
+  op iota_ : int -> int -> int list.
+
+  axiom iota0 i n : n <= 0 => iota_ i n = [].
+  axiom iotaS i n : 0 <= n => iota_ i (n+1) = i :: iota_ (i+1) n.
+
+  lemma iota1 i : iota_ i 1 = [i].
+  proof. by rewrite (iotaS i 0) // iota0. qed.
+
+  lemma size_iota m n: size (iota_ m n) = max 0 n.
+  proof. 
+    elim/Induction.natind: n m => [n hn|n hn ih] m.
+      by rewrite iota0 // max_lel.
+    rewrite iotaS //= ih max_ler // smt.
+  qed.
+ 
+  lemma iota_add m n1 n2 : 0 <= n1 => 0 <= n2 =>
+     iota_ m (n1 + n2) = iota_ m n1 ++ iota_ (m + n1) n2.
+  proof.
+    move=> ge0_n1 ge0_n2; elim n1 ge0_n1 m => /= [|n1 ge0_n1 ih] m.
+      by rewrite (iota0 m 0).
+    by rewrite addzAC !iotaS // 1:smt ih addzAC addzA.
+  qed.
+ 
+  lemma iotaSr i n : 0 <= n =>
+    iota_ i (n+1) = rcons (iota_ i n) (i+n).
+  proof. by move=> ge0_n; rewrite iota_add // iota1 cats1. qed.
+
+  lemma nth_iota m n i w: 0 <= i < n => nth w (iota_ m n) i = m + i.
+  proof.
+    case=> ge0_i lt_in; rewrite (_ : n = i + ((n-i-1)+1)) 1:smt.
+    rewrite iota_add // 1:smt nth_cat size_iota max_ler //=.
+    by rewrite iotaS // smt.
   qed.
 
-  lemma perm_cons: forall x (xs ys:'a list),
-    xs <-> ys =>
-    (x::xs) <-> (x::ys)
+  lemma iota_addl (m1 m2:int) n: iota_ (m1 + m2) n = map ((+) m1) (iota_ m2 n).
+  proof.
+    elim/Induction.natind: n m2 => [n hn|n hn ih] m2; 1: by rewrite !iota0.
+    by rewrite !iotaS // map_cons -addzA ih.
+  qed.
+ 
+  lemma mem_iota m n i : mem (iota_ m n) i <=> (m <= i /\ i < m + n).
+  proof.
+    elim/Induction.natind: n m => [n hn|n hn ih] m.
+      by rewrite iota0 // smt.  
+    by rewrite iotaS // in_cons ih smt.
+  qed.
+
+  lemma iota_uniq m n : uniq (iota_ m n).
+  proof.
+    elim/Induction.natind: n m => [n hn|n hn ih] m.
+      by rewrite iota0.
+    by rewrite iotaS // cons_uniq mem_iota ih // smt.
+  qed.
+
+  lemma last_iota k m n:
+    last k (Iota.iota_ m n) = if n <= 0 then k else m + n - 1.
+  proof.
+    elim/Induction.natind: n m k => [n hn|n hn ih] m k.
+      by rewrite iota0 hn.
+    by rewrite iotaS //= ih smt.
+  qed.
+end Iota.
+
+export Iota.
+
+(* -------------------------------------------------------------------- *)
+theory Range.
+  op range (m n : int) = iota_ m (n - m).
+
+  import Ring.IntID.
+
+  lemma range_geq (m n : int): n <= m => range m n = [].
+  proof. smt. qed.
+
+  lemma range_ltn (m n : int): m < n =>
+    range m n = m :: range (m+1) n.
+  proof. smt. qed.
+
+  lemma rangeS (m : int): range m (m+1) = [m].
+  proof. by rewrite range_ltn 1:smt range_geq. qed.
+
+  lemma range_add (m n a : int):
+    range (m+a) (n+a) = map (Int.(+) a) (range m n).
+  proof. by rewrite /range addrC iota_addl; congr; smt. qed.
+
+  lemma range_addl (m n a : int):
+    range (m+a) n = map (Int.(+) a) (range m (n-a)).
+  proof. by rewrite -{1}(addrNK a n) -subrE range_add. qed.
+
+  lemma range_addr (m n a : int):
+    range m (n+a) = map (Int.(+) a) (range (m-a) n).
+  proof. by rewrite -{1}(addrNK a m) -subrE range_add. qed.
+
+  lemma range_cat (n m p : int): m <= n => n <= p =>
+    range m p = range m n ++ range n p.
+  proof. 
+    rewrite /range (_: p - m = n - m + (p - n)) 1:smt.
+    by move=> le_mn le_np; rewrite iota_add; smt.
+  qed.
+
+  lemma mem_range (m n i: int):
+    (mem (range m n) i) <=> (m <= i < n).
+  proof.
+    rewrite /range mem_iota; case: (m <= i)=> //=.
+    by rewrite subrE addrCA addrN addr0.
+  qed.
+
+  lemma range_uniq m n: uniq (range m n).
+  proof. by apply/iota_uniq. qed.
+
+  lemma size_range m n: size (range m n) = max 0 (n - m).
+  proof. by apply/size_iota. qed.
+
+  lemma nth_range  (i p k w : int):
+    0 <= i < p - k => nth w (range k p) i = k + i.
+  proof. by apply/nth_iota. qed.
+end Range.
+
+export Range.
+
+(* -------------------------------------------------------------------- *)
+(*                        Association lists                             *)
+(* -------------------------------------------------------------------- *)
+op assoc (xs : ('a * 'b) list) (a : 'a) =
+  omap snd (onth xs (index a (map fst xs))).
+
+lemma assoc_nil a: assoc [<:'a * 'b>] a = None.
+proof. by []. qed.
+
+lemma assoc_cons x y s a:
+    assoc<:'a, 'b> ((x, y) :: s) a
+  = if a = x then Some y else assoc s a.
+proof.
+  rewrite /assoc /= index_cons {1 3}/fst /=; case: (a = x)=> //=.
+  by move=> _; rewrite addAzN addz1_neq0 // index_ge0.
+qed.
+
+lemma assoc_head x y s: assoc<:'a, 'b> ((x, y) :: s) x = Some y.
+proof. by rewrite assoc_cons. qed.
+
+lemma assoc_cat (s1 s2 : ('a * 'b) list) x:
+    assoc (s1 ++ s2) x
+  = if mem (map fst s1) x then assoc s1 x else assoc s2 x.
+proof.
+  elim: s1 => /= [|[x' y'] s ih] //; rewrite !assoc_cons /=.
+  by rewrite /(fst _) /=; case: (x = x').
+qed.
+
+lemma mem_assoc_uniq (s : ('a * 'b) list) (a : 'a) (b : 'b):
+  uniq (map fst s) => mem s (a, b) <=> assoc s a = Some b.
+proof.
+  elim: s => //= [[x y]] s ih; rewrite eq_sym => [x_notin_1s uq_1s] /=.
+  case: (x = a) => [->> |] /=; 1: rewrite assoc_head /=.
+    by apply/eq_iff/orb_idr=> /(map_f fst); rewrite x_notin_1s.
+  by move=> ne_xa; rewrite assoc_cons ih // @(eq_sym a) ne_xa.
+qed.
+
+lemma assocP (s : ('a * 'b) list) (x : 'a):
+     (  mem (map fst s) x /\ exists y, mem s (x, y) /\ assoc s x = Some y)
+  \/ (! mem (map fst s) x /\ assoc s x = None).
+proof.
+  elim: s=> //=; case=> x' y' s ih; rewrite /(fst (x', _)) /=.
+  case: (x = x') => /= [<<- |]; 1: by exists y'; rewrite assoc_cons.
+  by rewrite assoc_cons => ->.
+qed.
+
+lemma perm_eq_assoc (s1 s2 : ('a * 'b) list) x:
+     uniq (map fst s2)
+  => perm_eq s1 s2 => assoc s1 x = assoc s2 x.
+proof.
+  move=> uq_s1 peq_s1s2.
+  case: (assocP s1 x); last first.
+    case=> Ns1_x ->; case: (assocP s2 x); 2: by case=> _ <-.
+    by have/perm_eq_mem <- := perm_eq_map fst _ _ peq_s1s2.
+  case=> s1_x [y1 [s1_xy1 ->]]; apply/eq_sym.
+  by rewrite -mem_assoc_uniq //; apply/(perm_eq_mem _ _ peq_s1s2).
+qed.
+
+lemma assoc_filter (p : 'a -> bool) (s : ('a * 'b) list) x:
+  assoc (filter (p \o fst) s) x = if (p x) then assoc s x else None.
+proof.
+  elim: s=> //= [|[x' y'] s ih]; 1: by rewrite assoc_nil.
+  rewrite assoc_cons; case: (x = x') => [<<- |ne_xx'].
+    rewrite {1}/(\o) {1}/fst /=; case (p x).
+    by rewrite assoc_cons. by rewrite ih=> ->.
+  by case: ((\o) _ _ _)=> //=; rewrite assoc_cons ne_xx'.
+qed.
+
+(* -------------------------------------------------------------------- *)
+(*         Sequence from a function computing from indexes              *)
+(* -------------------------------------------------------------------- *)
+op mkseq (f : int -> 'a) n = map f (iota_ 0 n).
+
+lemma size_mkseq (f : int -> 'a) n: size (mkseq f n) = max 0 n.
+proof. by rewrite /mkseq size_map size_iota. qed.
+
+lemma eq_mkseq (f g : int -> 'a):
+     (forall x, f x = g x)
+  => forall n, mkseq f n = mkseq g n.
+proof. by move=> Efg n; apply eq_map. qed.
+
+lemma nth_mkseq x0 (f : int -> 'a) n i:
+  0 <= i < n => nth x0 (mkseq f n) i = f i.
+proof.
+  by move=> Hi; rewrite /mkseq (nth_map 0) ?nth_iota ?size_iota; smt.
+qed.
+
+lemma mkseq_nth (x0 : 'a) s: mkseq (nth x0 s) (size s) = s.
+proof.
+  apply (eq_from_nth x0); rewrite size_mkseq; first smt.
+  by move=> i Hi; rewrite nth_mkseq //; smt.
+qed.
+
+(* -------------------------------------------------------------------- *)
+(*                         Sequence folding                             *)
+(* -------------------------------------------------------------------- *)
+op foldr (f : 'a -> 'b -> 'b) z0 xs =
+  with xs = []      => z0
+  with xs = y :: ys => f y (foldr f z0 ys).
+
+lemma foldr_cat (f : 'a -> 'b -> 'b) z0 s1 s2:
+  foldr f z0 (s1 ++ s2) = foldr f (foldr f z0 s2) s1.
+proof. by elim s1 => //= x s1 ->. qed.
+
+lemma foldr_map ['a 'b 'c] (f : 'a -> 'b -> 'b) (h : 'c -> 'a) z0 s:
+  foldr f z0 (map h s) = foldr (fun x z, f (h x) z) z0 s.
+proof. by elim s => //= x s ->. qed.
+
+op foldl (f : 'b -> 'a -> 'b) z0 xs =
+  with xs = []      => z0
+  with xs = y :: ys => foldl f (f z0 y) ys.
+
+lemma foldl_rev (f : 'b -> 'a -> 'b) z0 s:
+  foldl f z0 (rev s) = foldr (fun x z => f z x) z0 s.
+proof.
+  elim/last_ind s z0 => [|s x ih] z0 /=; 1: by rewrite rev_nil.
+  by rewrite rev_rcons -cats1 foldr_cat -ih.
+qed.
+
+lemma foldl_cat (f : 'b -> 'a -> 'b) z0 s1 s2:
+  foldl f z0 (s1 ++ s2) = foldl f (foldl f z0 s1) s2.
+proof.
+  by rewrite -(revK (s1 ++ s2)) foldl_rev rev_cat foldr_cat -!foldl_rev !revK.
+qed.
+
+lemma foldr_perm (f : 'a -> 'b -> 'b) (z : 'b) (s1 s2 : 'a list):
+     (forall a b v, f a (f b v) = f b (f a v))
+  => perm_eq s1 s2
+  => foldr f z s1 = foldr f z s2.
+proof.
+  move=> fAC /perm_eqP; elim: s1 s2 => [|i s1 ih1] s2 eq_s12.
+    by case s2 eq_s12 => // i s2 h; cut := h (pred1 i); smt.
+  cut r2i: mem s2 i by rewrite -has_pred1 has_count -eq_s12 smt.
+  have/splitPr {r2i} [s3 s4] ->> := r2i; rewrite foldr_cat /=.
+  rewrite @(ih1 (s3 ++ s4)); 1: move=> p.
+    have /= := eq_s12 p; rewrite !count_cat /=.
+    by rewrite addzCA => /addzI.
+  rewrite foldr_cat => {eq_s12}; elim: s3 => [|x s3 ih2] //.
+  by rewrite /= fAC ih2.
+qed.
+
+lemma foldr_rem (x : 'a) (f : 'a -> 'b -> 'b) (z : 'b) (s : 'a list):
+     (forall a b X, f a (f b X) = f b (f a X))
+  => mem s x
+  => foldr f z s = f x (foldr f z (rem x s)).
+proof. by move=> fAC /perm_to_rem peq; rewrite @(foldr_perm f z _ _ fAC peq). qed.
+
+(* -------------------------------------------------------------------- *)
+(*                            Flattening                                *)
+(* -------------------------------------------------------------------- *)
+op flatten ['a] = foldr (++) [<:'a>].
+
+(* -------------------------------------------------------------------- *)
+(*                               EqIn                                   *)
+(* -------------------------------------------------------------------- *)
+lemma eq_in_filter p1 p2 (s : 'a list):
+     (forall x, mem s x => p1 x <=> p2 x)
+  => filter p1 s = filter p2 s.
+proof.
+  elim: s => //= x s ih eq_p; rewrite eq_p // ih //.
+  by move=> x' x'_in_s; apply/eq_p; rewrite x'_in_s.
+qed.
+
+(* -------------------------------------------------------------------- *)
+(*                         Sequence sorting                             *)
+(* -------------------------------------------------------------------- *)
+op path (e : 'a -> 'a -> bool) (x : 'a) (p : 'a list) : bool =
+  with p = []      => true
+  with p = y :: p' => e x y /\ path e y p'.
+
+op sorted (e : 'a -> 'a -> bool) (xs : 'a list) =
+  with xs = []      => true
+  with xs = y :: ys => path e y ys.
+
+theory InsertSort.
+  op insert (e : 'a -> 'a -> bool) (x : 'a) (s : 'a list) =
+    with s = []      => [x]
+    with s = y :: s' => if e x y then x :: s else y :: (insert e x s').
+
+  op sort (e : 'a -> 'a -> bool) (s : 'a list) =
+    with s = []      => []
+    with s = x :: s' => insert e x (sort e s').
+
+  lemma nosmt perm_insert (e : 'a -> 'a -> bool) x s:
+    perm_eq (x :: s) (insert e x s).
+  proof.
+    elim s => //= y s IHs; case (e x y) => exy.
+      by rewrite perm_cons perm_eq_refl.
+    by rewrite perm_consCA perm_cons.
+  qed.
+
+  lemma nosmt perm_sort (e : 'a -> 'a -> bool) s: perm_eq (sort e s) s.
+  proof.
+    elim s=> //= x s IHs; cut h := perm_insert e x (sort e s).
+    by apply perm_eqlE in h; rewrite -h perm_cons => {h}.
+  qed.
+
+  lemma nosmt sorted_insert (e : 'a -> 'a -> bool) x s:
+       (forall x y, e x y \/ e y x)
+    => sorted e s => sorted e (insert e x s).
+  proof.
+    move=> e_ltgt; case s => //= y s; case (e x y) => [-> -> // |].
+    elim s x y => /= [|z s IHs] x y; first by smt.
+    move=> Nexy [eyz pt_zs]; case (e x z); first by smt.
+    by move=> Nexz; rewrite eyz /= IHs.
+  qed.
+
+  lemma nosmt sort_sorted (e : 'a -> 'a -> bool) (s : 'a list):
+     (forall x y, e x y \/ e y x) => sorted e (sort e s).
+  proof. by move=> e_ltgt; elim s => //= x s IHs; apply sorted_insert. qed.
+end InsertSort.
+
+op sort (e : 'a -> 'a -> bool) s = InsertSort.sort e s axiomatized by sortE.
+
+lemma perm_sort e (s : 'a list): perm_eq (sort e s) s.
+proof. by rewrite sortE /=; apply InsertSort.perm_sort. qed.
+
+lemma sort_sorted (e : 'a -> 'a -> bool) s:
+  (forall (x y : 'a), e x y \/ e y x) => sorted e (sort e s).
+proof. by rewrite sortE /=; apply InsertSort.sort_sorted. qed.
+
+(* -------------------------------------------------------------------- *)
+(*                          Order lifting                               *)
+(* -------------------------------------------------------------------- *)
+op lex (e : 'a -> 'a -> bool) s1 s2 =
+  with s1 = []      , s2 = []       => true
+  with s1 = []      , s2 = y2 :: s2 => true
+  with s1 = y1 :: s1, s2 = []       => false
+  with s1 = y1 :: s1, s2 = y2 :: s2 =>
+    if e y1 y2 then if e y2 y1 then lex e s1 s1 else true else false.
+
+lemma lex_total (e : 'a -> 'a -> bool):
+     (forall x y, e x y \/ e y x)
+  => (forall s1 s2, lex e s1 s2 \/ lex e s2 s1).
+proof. by move=> h; elim=> [|x1 s1 IHs1] [|x2 s2] //=; smt. qed.
+
+(* -------------------------------------------------------------------- *)
+(*                          Array Notations                             *)
+(* -------------------------------------------------------------------- *)
+theory Array.
+  op "_.[_]" (s : 'a list) (n : int) = nth witness s n
+    axiomatized by getE.
+
+  op "_.[_<-_]" (s : 'a list) (n : int) (x : 'a) =
+    with s = []     => []
+    with s = a :: s => if n = 0 then x::s else a::(s.[n - 1 <- x]).
+
+  op mapi (n : int) (f : int -> 'a -> 'b) (s : 'a list) =
+    with s = []     => []
+    with s = x :: s => (f n x)::(mapi (n + 1) f s).
+
+  lemma nosmt arrayP (a1 a2 : 'a list):
+    (a1 = a2) <=>
+    (size a1 = size a2 /\ (forall i, 0 <= i < size a2 => a1.[i] = a2.[i])).
+  proof.
+    split=> [-> //= | []].
+    elim a2 a1=> /= [a1| x xs ih [//= | //= x' xs' /addzI eq_sizes h]].
+      by rewrite size_eq0=> ->.
+      by rewrite eq_sym addzC addz1_neq0 1:size_ge0.
+    split.
+      by have //= := h 0 _; rewrite ?getE //= -lez_add1r lez_addl size_ge0.
+    apply ih=> //.
+    move=> i [le0_i lti_lenxs]; have:= h (i + 1) _.
+      smt. (* side conditions... *)
+    by rewrite !getE /= addz1_neq0 //= addAzN.
+  qed.
+
+  lemma size_set (xs : 'a list) (n : int) (a : 'a):
+    size xs.[n <- a] = size xs.
+  proof. by elim xs n => //= x xs ih n; case (n = 0)=> //=; rewrite ih. qed.
+
+  lemma set_out (n : int) (a : 'a) (xs : 'a list):
+    n < 0 \/ size xs <= n =>
+    xs.[n <- a] = xs.
+  proof.
+    elim xs n=> //= x xs ih n; smt.
+(*    move=> h; have -> /=: n <> 0 by smt.
+    case {-1}(n < 0) (eq_refl (n < 0)) h=> //= [lt0_n | ].
+      by apply ih; left; smt.
+    rewrite neqF ltzNge /= => le0_n lt_xs_n.
+    by apply ih; right; smt. *)
+  qed.
+
+  lemma nth_set (n n': int) (a : 'a) (xs : 'a list):
+    0 <= n  < size xs =>
+    xs.[n <- a].[n'] = if n' = n then a else xs.[n'].
+  proof.
+    move=> n_bounds.
+    rewrite !getE; elim xs n n_bounds n'=> //=.
+      smt.
+    move=> x xs ih n n_bounds n'.
+    case (n = 0)=> //= [->> | ].
+      by case (n' = 0).
+    case (n' = 0)=> //= [->> | ne0_n' ne0_n].
+      by rewrite eq_sym=> ->.
+    by rewrite ih 1..2:smt.
+  qed. 
+
+  lemma get_set (xs : 'a list) (n n' : int) (x : 'a):
+    xs.[n <- x].[n'] =
+      if   (0 <= n < size xs /\ n' = n)
+      then x
+      else xs.[n']
   by [].
 
-  lemma perm_rm: forall x (xs ys:'a list),
-    xs <-> ys =>
-    (rm x xs) <-> (rm x ys).
-  proof strict.
-  intros=> x xs ys; case (mem x xs).
-    intros=> x_in_xs xs_ys; cut x_in_ys: mem x ys; first by rewrite -count_mem -(xs_ys x) count_mem //.
-    delta (<->) beta=> x'; case (x = x')=> x_x'.
-        subst x'; rewrite count_rm_in // count_rm_in // xs_ys //.
-        rewrite count_rm_neq // count_rm_neq // xs_ys //.
-    intros=> x_nin_xs xs_ys; cut x_nin_ys: !mem x ys; first by rewrite -count_mem -(xs_ys x) count_mem //.
-      delta (<->) beta=> x'; case (x = x')=> x_x'.
-        subst x'; rewrite count_rm_nin // count_rm_nin // xs_ys //.
-        rewrite count_rm_neq // count_rm_neq // xs_ys //.
-  qed.
+  lemma set_set (xs : 'a list) (n n' : int) (x x' : 'a):
+    forall i,
+      xs.[n <- x].[n' <- x'].[i] =
+        if   n = n'
+        then xs.[n' <- x'].[i]
+        else xs.[n' <- x'].[n <- x].[i]
+   by [].
 
-  lemma foldC: forall (x:'a) (f:'a -> 'b -> 'b) (z:'b) (xs:'a list),
-      (forall a b X, f a (f b X) = f b (f a X)) =>
-      mem x xs =>
-      foldr f z xs = f x (foldr f z (rm x xs)).
-  proof strict.
-  intros=> x f z xs C; elim/list_ind xs; first smt.
-    intros=> x' xs IH //=.
-    case (x' = x)=> x_x';first subst x';rewrite rm_consE //.
-    intros=> // x_in_xs.
-    by rewrite rm_consNE //= IH // C //.
-  qed.
+  lemma set_set_eq (xs : 'a list) (n : int) (x x' : 'a):
+    forall i, xs.[n <- x].[n <- x'].[i] = xs.[n <- x'].[i].
+  proof. by move=> i; rewrite set_set. qed.
 
-  lemma foldCA: forall (f:'a -> 'a -> 'a) (z x:'a) (xs:'a list),
-    (forall x y, f x y = f y x) =>
-    (forall x y z, f x (f y z) = f (f x y) z) =>
-    mem x xs =>
-    foldr f z xs = f x (foldr f z (rm x xs)).
-  proof strict.
-  intros f z x xs C A.
-  apply foldC=> a b c.
-  rewrite A (C a) -A //.
-  qed.
-
-  lemma fold_permC: forall (f:'a -> 'b -> 'b) (z:'b) (xs ys:'a list),
-    (forall a b X, f a (f b X) = f b (f a X)) =>
-    xs <-> ys =>
-    foldr f z xs = foldr f z ys.
-  proof strict.
-  intros=> f z xs ys C;generalize ys; elim/list_ind xs.
-    by intros=> ys nil_ys; rewrite (perm_nil ys); [apply perm_symm=> // | trivial ].
-    intros=> x xs IH ys xs_ys; rewrite (foldC x _ _ ys); first assumption.
-    rewrite -count_mem -xs_ys; smt.
-       cut rm_xs_ys: xs <-> rm x ys;
-         first by rewrite -(rm_consE x xs); apply perm_rm=> //.
-        rewrite //= (IH (rm x ys))=> //.
-  qed.
-
-  lemma fold_perm: forall (f:'a -> 'a -> 'a) (z:'a) (xs ys:'a list),
-    (forall x y, f x y = f y x) =>
-    (forall x y z, f x (f y z) = f (f x y) z) =>
-    xs <-> ys =>
-    foldr f z xs = foldr f z ys.
-  proof strict.
-  intros f z x xs C A.
-  apply fold_permC=> a b c.
-  rewrite A (C a) -A //.
-  qed.
-
-  (** Properties of unique lists up to permutation *)
-  lemma perm_unique: forall (xs ys:'a list),
-    xs <-> ys =>
-    unique xs =>
-    unique ys
-  by [].
-
-  lemma cons_nin: forall (x:'a) (xs ys:'a list),
-    unique ys =>
-    x::xs <-> ys =>
-    !mem x xs
-  by [].
-
-  lemma perm_length: forall (xs ys:'a list),
-    xs <-> ys =>
-    length xs = length ys.
-  proof strict.
-  intros=> xs; elim/list_ind xs.
-    smt.
-    intros=> x xs IH ys xs_ys //=.
-      rewrite (IH (rm x ys)).
-        by rewrite -(rm_consE x xs); apply perm_rm=> //. (* This should become a lemma *)
-        by rewrite length_rm; smt.
-  qed.
-end PermutationLists.
+  lemma get_mapi (f : int -> 'a -> 'b) (xs : 'a list) (n i : int):
+    0 <= n < size xs =>
+    (mapi i f xs).[n] = f (n + i) xs.[n].
+  proof. by rewrite !getE; elim xs i n=> //=;smt. qed.
+end Array.
